sch: style and reorg

src/sch/core.lean
@@ -2,65 +2,49 @@ import typ
 
 namespace tts ------------------------------------------------------------------
 
--- Grammar of type schemes.
+/-- Grammar of type schemes -/
 @[derive decidable_eq]
 structure sch (V : Type) : Type :=
-  (arity : ℕ)
-  (type : typ V)
+(arity : ℕ)
+(type : typ V)
 
 attribute [pp_using_anonymous_constructor] sch
 
-variables {V : Type} -- Type of variable names
-
 namespace sch ------------------------------------------------------------------
-variables [_root_.decidable_eq V]
+variables {V : Type} [_root_.decidable_eq V] -- Type of variable names
+variables {a : ℕ} -- Type scheme arity
+variables {x : tagged V} -- Variables
+variables {xs : list (tagged V)} -- List of variables
+variables {t tx : typ V} -- Types
+variables {ts txs : list (typ V)} -- Lists of types
 
 theorem eq_of_veq : ∀ {s₁ s₂ : sch V}, s₁.arity = s₂.arity → s₁.type = s₂.type → s₁ = s₂
 | ⟨a₁, t₁⟩ ⟨a₂, t₂⟩ ha ht := by congr; solve_by_elim
 
--- Get the free variables of a scheme.
+/-- Get the free variables of a scheme -/
 def fv (s : sch V) : finset (tagged V) :=
-  typ.fv s.type
+typ.fv s.type
 
-@[simp]
-theorem fv_mk {a : ℕ} {t : typ V} : fv (mk a t) = typ.fv t :=
-  rfl
+@[simp] theorem fv_mk : fv (mk a t) = typ.fv t :=
+rfl
 
--- Substitute a free variable for a type in a scheme
-def subst (x : tagged V) (t : typ V) (s : sch V) : sch V :=
-  ⟨s.arity, typ.subst x t s.type⟩
-
-@[simp]
-theorem subst_mk {a : ℕ} {x : tagged V} {tx t : typ V} : subst x tx (mk a t) = mk a (typ.subst x tx t) :=
-  rfl
-
--- Substitute a list of free variables for a list of types in a scheme
-def subst_list (xs : list (tagged V)) (ts : list (typ V)) (s : sch V) : sch V :=
-  ⟨s.arity, typ.subst_list xs ts s.type⟩
-
-@[simp]
-theorem subst_list_mk {a : ℕ} {xs : list (tagged V)} {ts : list (typ V)} {t : typ V} : subst_list xs ts (mk a t) = mk a (typ.subst_list xs ts t) :=
-  rfl
-
--- Open a type scheme with a list of types for bound variables.
+/-- Open a type scheme with a list of types for bound variables -/
 def open_typs (ts : list (typ V)) (s : sch V) : typ V :=
-  typ.open_typs ts s.type
+typ.open_typs ts s.type
 
-@[simp]
-theorem open_typs_mk {ts : list (typ V)} {a : ℕ} {t : typ V} : open_typs ts (mk a t) = typ.open_typs ts t :=
-  rfl
+@[simp] theorem open_typs_mk : open_typs ts (mk a t) = typ.open_typs ts t :=
+rfl
 
--- Open a type scheme with a list of free variables for bound variables.
+/-- Open a type scheme with a list of free variables for bound variables -/
 def open_vars (xs : list (tagged V)) (s : sch V) : typ V :=
-  typ.open_vars xs s.type
+typ.open_vars xs s.type
 
-@[simp]
-theorem open_vars_mk {xs : list (tagged V)} {a : ℕ} {t : typ V} : open_vars xs (mk a t) = typ.open_vars xs t :=
-  rfl
+@[simp] theorem open_vars_mk : open_vars xs (mk a t) = typ.open_vars xs t :=
+rfl
 
--- A scheme is locally-closed if its body is locally closed.
+/-- Locally-closed type scheme -/
 def lc (s : sch V) : Prop :=
-  typ.lc_body s.arity s.type
+typ.lc_body s.arity s.type
 
 end /- namespace -/ sch --------------------------------------------------------
 end /- namespace -/ tts --------------------------------------------------------
