src/sch/subst.lean
@@ -1,68 +1,78 @@
 import .core
-import typ
 
 namespace tts ------------------------------------------------------------------
 namespace sch ------------------------------------------------------------------
-variables {n : ℕ} -- Natural numbers
-variables {V : Type} -- Type of variable names
+variables {V : Type} [_root_.decidable_eq V] -- Type of variable names
+variables {a : ℕ} -- Type scheme arity
 variables {x x₁ x₂ : tagged V} -- Variables
 variables {xs : list (tagged V)} -- List of variable names
-variables {t t₁ t₂ : typ V} -- Types
-variables {ts : list (typ V)} -- Lists of types
-variables {s : sch V} -- Schemes
+variables {t tx t₁ t₂ : typ V} -- Types
+variables {ts txs : list (typ V)} -- Lists of types
+variables {s : sch V} -- Type schemes
 
-variables [_root_.decidable_eq V]
+open list
+
+/-- Substitute a free variable for a type in a scheme -/
+def subst (x : tagged V) (t : typ V) (s : sch V) : sch V :=
+⟨s.arity, typ.subst x t s.type⟩
+
+@[simp] theorem subst_mk : subst x tx (mk a t) = mk a (typ.subst x tx t) :=
+rfl
+
+/-- Substitute a list of free variables for a list of types in a scheme -/
+def subst_list (xs : list (tagged V)) (ts : list (typ V)) (s : sch V) : sch V :=
+⟨s.arity, typ.subst_list xs ts s.type⟩
+
+@[simp] theorem subst_list_mk :
+  subst_list xs txs (mk a t) = mk a (typ.subst_list xs txs t) :=
+rfl
 
 -- Substitution with a fresh name is the identity
-@[simp]
-theorem subst_fresh (h : x ∉ fv s) : subst x t s = s :=
-  eq_of_veq rfl $ typ.subst_fresh h
+@[simp] theorem subst_fresh (h : x ∉ fv s) : subst x t s = s :=
+eq_of_veq rfl $ typ.subst_fresh h
 
 -- Fold typ.subst into sch.subst
-theorem subst_fold : mk n (typ.subst x t₂ t₁) = subst x t₂ (mk n t₁) :=
-  rfl
+theorem subst_fold : mk a (typ.subst x t₂ t₁) = subst x t₂ (mk a t₁) :=
+rfl
 
 -- Substitution distributes over open
-theorem subst_open_typs (l : typ.lc t)
-: typ.subst x t (open_typs ts s) = open_typs (list.map (typ.subst x t) ts) (subst x t s) :=
-  by cases s; simp [typ.subst_open_typs l]
+theorem subst_open_typs (l : typ.lc t) :
+  typ.subst x t (open_typs ts s) = open_typs (map (typ.subst x t) ts) (subst x t s) :=
+by cases s; simp [typ.subst_open_typs l]
 
 -- Substitution distributes over open_vars
-theorem subst_open_vars (h : x ∉ xs) (l : typ.lc t)
-: open_vars xs (subst x t s) = typ.subst x t (open_vars xs s) :=
-  by cases s; simp [typ.subst_open_vars h l]
+theorem subst_open_vars (h : x ∉ xs) (l : typ.lc t) :
+  open_vars xs (subst x t s) = typ.subst x t (open_vars xs s) :=
+by cases s; simp [typ.subst_open_vars h l]
 
-@[simp]
-theorem subst_arity : (subst x t s).arity = s.arity :=
-  by unfold subst
+@[simp] theorem subst_arity : (subst x t s).arity = s.arity :=
+by unfold subst
 
-@[simp]
-theorem subst_type : (subst x t s).type = typ.subst x t s.type :=
-  by unfold subst
+@[simp] theorem subst_type : (subst x t s).type = typ.subst x t s.type :=
+by unfold subst
 
 -- A scheme substituted with a type is well-formed if the scheme is well-formed
 -- and the type is locally-closed.
 theorem subst_well_formed (lt : typ.lc t) (ls : lc s) : lc (subst x t s) :=
-  begin
-    cases ls with L ls,
-    existsi insert x L,
-    intros xs d ln_eq F,
-    simp [not_or_distrib] at F,
-    have h₁ : x ∉ xs := λ h, absurd (eq.refl x) (F h).1,
-    have h₂ : ∀ x ∈ xs, x ∉ L := λ _ h, (F h).2,
-    simp [typ.subst_open_vars h₁ lt, typ.subst_lc lt (ls d ln_eq h₂)],
-  end
+begin
+  cases ls with L ls,
+  existsi insert x L,
+  intros xs d ln_eq F,
+  simp [not_or_distrib] at F,
+  have h₁ : x ∉ xs := λ h, absurd (eq.refl x) (F h).1,
+  have h₂ : ∀ x ∈ xs, x ∉ L := λ _ h, (F h).2,
+  simp [typ.subst_open_vars h₁ lt, typ.subst_lc lt (ls d ln_eq h₂)],
+end
 
 -- Opening up a scheme `s` with `ts` is the same as opening up `s` with fresh
 -- names `xs` and then substituting `xs` for `ts`.
 theorem subst_list_intro
-(d : xs.nodup)
-(ln_eq : xs.length = ts.length)
-(F : ∀ x ∈ xs, x ∉ fv s ∪ typ.fv_list ts)
-(l : ∀ t ∈ ts, typ.lc t)
-: open_typs ts s = typ.subst_list xs ts (open_vars xs s) :=
-  by unfold open_typs open_vars;
-     exact typ.subst_list_intro d ln_eq F l
+  (d : xs.nodup)
+  (ln_eq : xs.length = ts.length)
+  (F : ∀ x ∈ xs, x ∉ fv s ∪ typ.fv_list ts)
+  (l : ∀ t ∈ ts, typ.lc t) :
+  open_typs ts s = typ.subst_list xs ts (open_vars xs s) :=
+by unfold open_typs open_vars; exact typ.subst_list_intro d ln_eq F l
 
 end /- namespace -/ sch --------------------------------------------------------
 end /- namespace -/ tts --------------------------------------------------------
