src/sch/open.lean
@@ -1,36 +1,34 @@
 import .core
-import typ
 
 namespace tts ------------------------------------------------------------------
 namespace sch ------------------------------------------------------------------
-variables {V : Type} -- Type of variable names
-variables [_root_.decidable_eq V]
+variables {V : Type} [_root_.decidable_eq V] -- Type of variable names
 variables {ts : list (typ V)} -- Lists of types
-variables {s : sch V} -- Schemes
+variables {s : sch V} -- Type schemes
 
 -- A locally-closed schema opened with a list of types is locally-closed if all
 -- types are locally-closed.
-theorem open_lc
-(v : V)
-(ls : lc s)
-(ln_eq_s : s.arity = ts.length)
-(lts : ∀ t ∈ ts, typ.lc t)
-: typ.lc (open_typs ts s) :=
-  begin
-    cases ls with L ls,
-    let L' := fv s ∪ typ.fv_list ts ∪ L,
-    let FL' := ((fresh.tagged v).pgenl L' ts.length).1,
-    have dL' : FL'.nodup := (fresh.tagged v).pgenl_nodup L' ts.length,
-    have ln_eq_FL' : FL'.length = ts.length :=
-      (fresh.tagged v).pgenl_length L' ts.length,
-    have Fs_ts : ∀ x ∈ FL', x ∉ typ.fv s.type ∪ typ.fv_list ts :=
-      λ _ h, ((fresh.tagged v).pgenl_mem_union h).1,
-    have FL : ∀ x ∈ FL', x ∉ L :=
-      λ _ h, ((fresh.tagged v).pgenl_mem_union h).2,
-    unfold open_typs,
-    rw typ.subst_list_intro dL' ln_eq_FL' Fs_ts lts,
-    exact typ.subst_list_lc ln_eq_FL' lts (ls dL' (ln_eq_FL'.trans ln_eq_s.symm) FL)
-  end
+theorem lc_open_typs
+  (v : V)
+  (ls : lc s)
+  (ln_eq_s : s.arity = ts.length)
+  (lts : ∀ t ∈ ts, typ.lc t) :
+  typ.lc (open_typs ts s) :=
+begin
+  cases ls with L ls,
+  let L' := fv s ∪ typ.fv_list ts ∪ L,
+  let FL' := ((fresh.tagged v).pgenl L' ts.length).1,
+  have dL' : FL'.nodup := (fresh.tagged v).pgenl_nodup L' ts.length,
+  have ln_eq_FL' : FL'.length = ts.length :=
+    (fresh.tagged v).pgenl_length L' ts.length,
+  have Fs_ts : ∀ x ∈ FL', x ∉ typ.fv s.type ∪ typ.fv_list ts :=
+    λ _ h, ((fresh.tagged v).pgenl_mem_union h).1,
+  have FL : ∀ x ∈ FL', x ∉ L :=
+    λ _ h, ((fresh.tagged v).pgenl_mem_union h).2,
+  unfold open_typs,
+  rw typ.subst_list_intro dL' ln_eq_FL' Fs_ts lts,
+  exact typ.subst_list_lc ln_eq_FL' lts (ls dL' (ln_eq_FL'.trans ln_eq_s.symm) FL)
+end
 
 end /- namespace -/ sch --------------------------------------------------------
 end /- namespace -/ tts --------------------------------------------------------
